:recycle: move to lecture 7, restructure

lecture6/lecture.dfy
@@ -271,7 +271,7 @@ method TestAbs()
 */
 
 method AbsFixed(x: int) returns (y: int)
-  // TODO: Fixed postcondition:
+  // Fixed postcondition:
   ensures y >= 0
   ensures y == x || y == -x
   // The interface is complete! The contract fully specifies
@@ -565,7 +565,7 @@ method Main()
 
 method StrongestPostconditionEx(x: int) returns (y: int)
   requires x >= 5
-  // TODO: what ensures statement should go here?
+  // What ensures statement should go here?
   ensures y == abs(x + x)
   ensures y >= 10
   ensures x >= 5
@@ -574,7 +574,7 @@ method StrongestPostconditionEx(x: int) returns (y: int)
 }
 
 method WeakestPreconditionEx(x: int) returns (y: int)
-  // TODO: what requires statement should go here?
+  // What requires statement should go here?
   // requires false // Replace this line
   requires x >= 5 || x <= -5
   ensures y >= 10
@@ -583,6 +583,32 @@ method WeakestPreconditionEx(x: int) returns (y: int)
 }
 
 // ##### Where we left off for day 20 #####
+
+/*
+  ===== Day 21 =====
+
+  Announcements:
+
+  - HW4 is released! Due Monday, June 3
+
+  - Installation instructions have been updated in the homework
+    README file. However, an important change: you don't need
+    the Dafny command line to complete the homework. You onlly
+    need the Dafny VSCode extension (with the green bars on the side).
+
+  - Looking ahead:
+    **Class on Friday, May 31 will be via Zoom.**
+    My office hours that week will be moved to Wednesday.
+    That way, leading up to the deadline you will have
+    Wednesday, Friday, and Monday office hours.
+
+  Plan for today:
+
+  - Poll
+  - Finish strongest postconditions and weakest preconditions
+  - Misc: sequences
+  - Move on to Lecture 7: loop invariants!
+*/
 
 // What about this? (A harder one)
 method StrongestPostconditionEx2(x: int) returns (y: int)
@@ -602,313 +628,8 @@ method StrongestPostconditionEx2(x: int) returns (y: int)
   Dafny works internally -- it is calculating them implicitly all the time!
 
   The way it does it is basically the process we did above.
+  It can be done in a completely routine way.
 
-  The process of fixing Abs and Double -- in order to make the
-  postcondition as strong as possible, so the test passes --
-  was basically about finding the strongest postcondition for the
-  method.
+  In fact, this process is also a super useful tool for debugging
+  to see where the Dafny verifier is getting stuck.
 */
-
-/*
-  ===== Recursion and loops =====
-
-  So far, the examples we've seen are quite simple; we could have done any
-  of this in Z3 pretty easily!
-
-  Loops and recursion is where program verifiers become both
-  much more powerful (expressive) -- and more effort-intensive.
-
-  Let's start with recursion:
-  Functions support recursion and can appear in expressions!
-
-  Let's define a function that computes a given fibonaci number:
-*/
-function fib(n: nat): nat
-{
-  if n == 0 then 0
-  else if n == 1 then 1
-  else fib(n-1) + fib(n-2)
-}
-
-/*
-  This function would be really slow due to recomputations if implemented as is,
-  so let's implement a fast method, and prove that it is equivalent.
-
-  We first need a loop, and then we will see one of the main very important notions of verification: loop invariants.
-
-  ===== Loop invariants =====
-
-  What is a loop invariant?
-
-  A loop invariant is an assertion that must hold
-  after *every* loop iteration. Like this:
-
-    assert <invariant>;
-    while P {
-      <loop body>
-      assert <invariant>;
-    }
-
-  Loop invariants are the key to verifying real-world code,
-  and they are often the hardest part to come up with.
-  We need to "guess" an invariant that both
-  (i) is satisfied before the loop runs
-  (ii) is preserved by the loop
-  (iii) is strong enough to prove what we want after the loop
-*/
-
-method ComputeFib(n: nat) returns (b: nat)
-  // ensures b == fib(n)
-{
-  if (n <= 0)
-  {
-    return n;
-  }
-  else
-  {
-    var prev := 0;
-    var curr := 1;
-
-    var i := 1;
-    while i < n
-      // invariant ...
-    {
-      curr, prev := curr + prev, curr;
-      i := i + 1;
-    }
-    return curr;
-  }
-}
-
-/*
-  ===== Termination =====
-
-  There's another thing that's implicitly going on with recursion and while loops:
-  program termination.
-
-  Exercise: add a decreases clause to both functions.
-
-  What does the decreases clause ensure?
-*/
-
-/*
-  ===== Another digression: the limits of verification? =====
-
-  Let's take a step back and consider what we've done so far.
-  - We managed to write a function to calculate Fibonacci numbers and
-    *prove* that it's always correct, on all inputs. Without ever running
-    the code.
-
-  - It was a bit difficult though: we had to come up with a special "loop invariant"
-    and (in theory) a "decreases" clause to make it work,
-    and the code wouldn't verify otherwise.
-    So is this always possible?
-
-  There's sort of an argument for NO and an argument for YES.
-
-  NO: Some of you may have heard that proving general properties
-  about programs is supposed to be impossible!
-  (It's OK if you haven't heard this.) For example,
-  we know that the halting problem is impossible to decide:
-
-    HALT(x) = "Does program x halt?"
-
-  There's no program which decides the above!
-  Yet, Dafny is able to determine not just that all the programs halt,
-  but that they are correct (satisfy the spec) on all inputs.
-  So in Dafny, we could decide the halting problem this way:
-
-    HALT(x): return true;
-
-  Let's take a minute to appreciate what that means: using just some math
-  equations and formulas, and a fancy verification tool (which uses Z3),
-  we know (without running it) that the program will give the correct
-  answer on **all possible inputs.** Not just some particular
-  inputs that we tried. It's a way to completely fool-proof all future uses
-  of the code.
-
-  YES: The surprising thing (at least if you've taken theory of computation)
-  is that in practice, yes, it is almost always possible to prove that
-  programs correct.
-
-  People have even built entire software projects: like cryptographic libraries,
-  operating system kernels, and (famously) an optimizing C compiler (CompCert)
-  entirely in formally verified programming languages.
-    https://sel4.systems/About/
-    https://compcert.org/
-
-  If program termination and correctness is undecidable in general, then how
-  are these projects possible?
-
-  Any ideas? :)
-
-  Answer:
-*/
-
-/*
-  ===== Arrays =====
-
-  Dafny supports imperative arrays. The only difference with C is that the array has its length in the data structure.
-*/
-
-method Find(a: array<int>, key: int) returns (index: int)
-  ensures 0 <= index < a.Length ==> (index < a.Length && a[index] == key)
-  ensures index == a.Length ==> forall k :: 0 <= k < a.Length ==> a[k] != key
-{
-  // Can we write code that satisfies the postcondition?
-  index := 0;
-  while (index < a.Length) && (a[index] != key)
-    decreases a.Length - index
-    invariant 0 <= index <= a.Length
-    invariant forall j : nat :: j < index ==> a[j] != key
-  {
-    // if a[index] == key
-    // {
-    //    return ;
-    // }
-    index := index + 1;
-  }
-  // index := -1;
-  // return -1;
-}
-
-// If we have time we can also look at this FindMax
-// method FindMax(a: array<int>) returns (max_i: int)
-//    requires a.Length > 0
-//    ensures 0 <= max_i < a.Length
-//    ensures forall k :: 0 <= k < a.Length ==> a[max_i] >= a[k]
-// {
-
-// }
-
-// Our postconditions and invariants are starting to grow big
-//   (especially when dealing with arrays)
-//   and so we would like to abstract away parts of them.
-//
-// For that, we can use predicates, i.e., boolean functions that can only be used in specifications.
-
-// Let's write a predicate that holds if its input array is sorted.
-
-predicate sorted(a: array<int>)
-  reads a // Necessary to give ownership to a predicate (or function) to read/write an array
-{
-  forall i, j :: 0 <= i < j < a.Length ==> a[i] <= a[j]
-}
-
-// And now to gather everything that we have seen in the lecture already,
-//   let's write the spec for a binary search, and then implement and verify it.
-//
-// We will go through the whole process, debugging whatever might go wrong etc.
-method BinarySearch(a: array<int>, value: int) returns (index: int)
-  requires sorted(a)
-  // modifies a
-  // During the lecture: Write pre and postconditions
-  ensures 0 <= index ==> (index < a.Length && a[index] == value)
-  ensures 0 > index ==> forall k :: 0 <= k < a.Length ==> a[k] != value
-{
-  // inclusive low, exclusive high
-  var low := 0;
-  var high := a.Length;
-
-  while low < high
-    decreases high - low
-    invariant 0 <= low <= high <= a.Length
-    invariant forall j :: 0 <= j < low ==> a[j] < value
-    invariant forall j :: high <= j < a.Length ==> a[j] > value
-    invariant sorted(a)
-  {
-
-    var i := (high + low) / 2;
-    if a[i] > value
-    {
-      high := i;
-    }
-    else if a[i] < value
-    {
-      low := i + 1;
-      var temp_ai := a[i];
-      assert forall j :: high <= j < a.Length ==> a[j] > value;
-      assert low > 0 ==> a[low - 1] < value;
-      assert forall j :: 0 <= j < low ==> a[j] < value;
-    }
-    else
-    {
-      return i;
-    }
-  }
-  return -1;
-}
-
-//
-// Allocating arrays
-//
-
-// Until now for simplicity we haven't shown any array allocation, but Dafny allows that too with the `new` keyword.
-
-method Copy(a: array<int>) returns (b: array<int>)
-{
-  b := new int[a.Length];
-}
-
-//
-// Sequences
-//
-
-// I will now give a brief overview of sequences to show how they facilitate verification.
-//   For a more complete reference see: (https://www.dcc.fc.up.pt/~nam/web/resources/vfs20/DafnyQuickReference.pdf)
-
-// Let's say we wanted to write a predicate that holds if a slice of the array was sorted
-
-predicate sorted_slice(a: array<int>, start: int, end: int)
-  reads a
-  requires 0 <= start < end < a.Length
-{
-  forall i,j :: start <= i < j < end ==> a[i] <= a[j]
-}
-
-// yuck
-
-// Sequences can help by allowing for easy slicing and slightly more succint syntax.
-//   Also they are immutable meaning that Dafny doesn't need to care about whether they are modified or not.
-
-
-predicate sorted_seq(a: seq<int>)
-{
-  forall i, j :: 0 <= i < j < |a| ==> a[i] <= a[j]
-}
-
-// And let's use it
-
-method TestSeq(a: array<int>)
-  // requires sorted_seq(a[0..10])
-{
-
-}
-
-//
-// Auxiliary State
-//
-
-// The final thing that one needs to know for the homework is that often
-//   the implementation code is not adequate for dafny to verify postconditions
-//   (especially in the presence of loops).
-//
-// In addition to the original code and state, there is often need for
-//   extra auxiliary state (variables, arrays) that can help establish a fact that is needed for a postcondition.
-//
-// An example of such extra state that might be helpful is a data structure that "logs" some important actions
-//   that were done in the loop.
-
-// And finishing with a quote from the official dafny tutorial
-//
-// ```
-//    Even if you do not use Dafny regularly, the idea of writing down exactly
-//    what it is that the code does in a precise way, and using this to prove code correct
-//    is a useful skill. Invariants, pre- and postconditions, and annotations are useful
-//    in debugging code, and also as documentation for future developers. When modifying
-//    or adding to a codebase, they confirm that the guarantees of existing code are not broken.
-//    They also ensure that APIs are used correctly, by formalizing behavior and requirements
-//    and enforcing correct usage. Reasoning from invariants, considering pre- and postconditions,
-//    and writing assertions to check assumptions are all general computer science skills
-//    that will benefit you no matter what language you work in.
-// ```
