lecture6/example.dfy
@@ -13,6 +13,7 @@
 method Abs(x: int) returns (y: int)
   requires true
   ensures y >= 0
+  ensures y == x || y == -x
 {
   if x >= 0 {
     return x;
