lecture7/repeated_squares.dfy
@@ -1,0 +1,25 @@
+/*
+  A harder exercise:
+  Implement a function that calculates
+  pow(x, n) = x^n
+
+  in a more efficient way than just multiplying x by itself n times.
+*/
+
+// Here is the easy recursive version.
+// We want to write a more efficient version.
+function power(x: int, pow: nat): int
+{
+  if pow == 0 then 1 else x * power(x, pow - 1)
+}
+
+// Lemmas
+/* TODO: add lemmas here as needed */
+
+method RepeatedSquare(x: int, pow: nat) returns (y: int)
+  ensures y == power(x, pow)
+  // TODO: Uncomment to implement the function
+  requires false
+{
+  // TODO
+}
