lecture7/README.md
@@ -1,0 +1,10 @@
+# Formal Verification 2: Loops and Recursion
+
+A.k.a.: Verifying general code with loop invariants!
+
+## Resources (updated)
+
+- [Dafny tutorial](https://dafny.org/latest/OnlineTutorial/guide)
+- [Dafny cheat sheet](https://dafny.org/latest/DafnyCheatsheet.pdf)
+- [Dafny reference manual and user guide](https://dafny.org/latest/DafnyRef/DafnyRef)
+- Textbook: *Program Proofs,* by Rustan M. Leino -- [link](https://mitpress.mit.edu/9780262546232/program-proofs/)
